confluence_of_lambda_calculus_according_to_takahashi.v
@@ -1,0 +1,695 @@
+Require Import NasLC.nested_abstract_syntax_lambda_calculus.
+
+(** This text proves the confluence of the lambda calculus with the method of parallel 
+    reductions invented by Masako Takahashi. We deal with beta eta reduction. 
+ The simpler other reductions have obviously the same proof but shorter. *)
+
+Section Takahashi_reductions_and_their_confluence.
+
+  Notation T:= Lambda_Term.
+  Notation V:= lt_var.
+  Notation A:= lt_app.
+  Notation L:= lt_abs.
+  Notation "^ C":= (option C) (right associativity, at level 41).
+  
+  Inductive parallel_beta_eta_direct_reduction (C:Set): T C -> T C -> Set:=
+  |pbed_var_refl: forall (x:C), parallel_beta_eta_direct_reduction C (V C x) (V C x)
+  |pbed_app: forall (a a' b b':T C),
+      parallel_beta_eta_direct_reduction C a a' ->
+      parallel_beta_eta_direct_reduction C b b' ->
+      parallel_beta_eta_direct_reduction C (A C a b) (A C a' b')
+  |pbed_abs: forall (f f':T (^C)),
+      parallel_beta_eta_direct_reduction (^C) f f' ->
+      parallel_beta_eta_direct_reduction C (L C f) (L C f')
+  |pbed_beta: forall (f f':T (^C)) (x x':T C),
+      parallel_beta_eta_direct_reduction (^C) f f' ->
+      parallel_beta_eta_direct_reduction C x x' ->
+      parallel_beta_eta_direct_reduction C (A C (L C f) x) (lt_specify_new_var C f' x')
+  |pbed_eta: forall (f f':T C),
+      parallel_beta_eta_direct_reduction C f f' ->
+      parallel_beta_eta_direct_reduction
+        C
+        (L C (A (^C) (lt_constant_embedding C f) (V (^C) None)))
+        f'.
+
+  Inductive parallel_beta_eta_reduction (C:Set): T C -> T C -> Set:=
+  |pbe_refl: forall (x: T C), parallel_beta_eta_reduction C x x
+  |pbe_step: forall (x y z:T C),
+      parallel_beta_eta_reduction C x y ->
+      parallel_beta_eta_direct_reduction C y z ->
+      parallel_beta_eta_reduction C x z.
+
+  Fixpoint pbed_refl (C:Set) (x:T C) {struct x}: parallel_beta_eta_direct_reduction C x x:=
+    match x as l return (parallel_beta_eta_direct_reduction C l l) with
+    | V _ c => pbed_var_refl C c
+    | A _ x1 x2 => pbed_app C x1 x1 x2 x2 (pbed_refl C x1) (pbed_refl C x2)
+    | L _ x0 => pbed_abs C x0 x0 (pbed_refl (^ C) x0)
+    end.
+
+  Notation "a §[ C ] b":= (parallel_beta_eta_direct_reduction C a b) (at level 49).
+  Notation "a §*[ C ] b":= (parallel_beta_eta_reduction C a b) (at level 49).
+  
+  Section Takahashi_reduction_with_change_of_variables_and_substitution.
+
+    Definition lt_constant_embedding_cov (C D:Set) (env: C -> D)
+               (f: T C):
+      lt_change_of_variables (^C) (lt_constant_embedding C f) (^D) (option_map env) =
+      lt_constant_embedding D (lt_change_of_variables C f D env).
+    Proof.
+      unfold lt_constant_embedding. repeat rewrite lt_cov_composition_equality.
+      simpl; reflexivity.
+    Defined.
+    
+    Definition pbed_cov (C:Set) (x y:T C) (r: x §[C] y):
+      forall (D:Set) (env: C -> D),
+      (lt_change_of_variables C x D env) §[D] (lt_change_of_variables C y D env).
+    Proof.
+      induction r. intros; simpl; apply pbed_var_refl.
+      intros; simpl; apply pbed_app. apply IHr1. apply IHr2.
+      intros; simpl; apply pbed_abs; apply IHr.
+      intros. rewrite lt_specify_new_var_cov. simpl. apply pbed_beta. apply IHr1. apply IHr2.
+      intros. simpl; rewrite lt_constant_embedding_cov. apply pbed_eta; apply IHr.
+    Defined.
+
+    Notation ce:= (lt_constant_embedding).
+    
+    Definition pbed_ce (C:Set) (x y:T C) (r: x §[C] y): (ce C x) §[^C] (ce C y):=
+      pbed_cov C x y r (^ C) Some.
+
+    Definition lt_constant_embedding_sub (C D:Set) (env: C -> T D)
+               (f: T C):
+      lt_substitution (^C) (lt_constant_embedding C f) (^D) (lt_extend_environment C D env) =
+      lt_constant_embedding D (lt_substitution C f D env).
+    Proof.
+      unfold lt_constant_embedding. unfold lt_extend_environment.
+      rewrite lt_sub_after_cov_equality. rewrite lt_cov_after_sub_equality.
+      apply lt_sub_pointwise_equality. unfold lt_constant_embedding; intro; reflexivity.
+    Defined.
+    
+    Definition pbed_sub (C:Set) (x y:T C) (r: x §[C] y):
+      forall (D:Set) (env1 env2: C -> T D) (redenv: forall i:C, env1 i §[D] env2 i),
+      (lt_substitution C x D env1) §[D] (lt_substitution C y D env2).
+    Proof.
+      induction r. intros; simpl; apply redenv. intros; simpl; apply pbed_app.
+      apply IHr1; assumption. apply IHr2; assumption.
+      intros; simpl; apply pbed_abs; apply IHr. intros. destruct i.
+      simpl; apply pbed_ce; apply redenv. simpl; apply pbed_var_refl.
+      intros. rewrite lt_specify_new_var_sub. simpl. apply pbed_beta. apply IHr1.
+      intros. destruct i. simpl; apply pbed_ce; apply redenv. simpl; apply pbed_var_refl.
+      apply IHr2; assumption.
+      intros. simpl. rewrite lt_constant_embedding_sub. apply pbed_eta. apply IHr; assumption.
+    Defined.      
+
+    Definition pbed_specify_new_var (C:Set) (f f': T (^C)) (x x':T C):
+      f §[^C] f' -> x §[C] x' -> lt_specify_new_var C f x §[C] lt_specify_new_var C f' x'.
+    Proof.
+      intros; unfold lt_specify_new_var; apply pbed_sub. assumption.
+      intros; destruct i; simpl. apply pbed_var_refl. assumption.
+    Defined.      
+      
+  End Takahashi_reduction_with_change_of_variables_and_substitution.
+  
+  Section the_maximum_direct_reduction_operator.
+
+
+    Section free_new_variables_and_constant_terms_characterizations.
+      
+      Fixpoint lt_free_variable_test (C:Set) (x:T C) {struct x}:
+        forall (v:C) (eqv: forall w:C, sumbool (v = w) (v <> w)),
+          sumbool (lt_free_variable C v x) (~ lt_free_variable C v x).
+      Proof.
+        destruct x. intros. destruct (eqv c). rewrite e. left; apply ltfv_atom.
+        right. intro F. inversion F. contradiction.
+        intros. destruct (lt_free_variable_test C x1 v eqv) as [y1|n1]. left.
+        apply ltfv_app_left; assumption.
+        destruct (lt_free_variable_test C x2 v eqv) as [y2|n2]. left.
+        apply ltfv_app_right; assumption. right. intro F. inversion F; contradiction.
+        intros. destruct lt_free_variable_test with (C:=^C) (x:=x) (v:= Some v) as [y|n].
+        intros. destruct w. destruct (eqv c). rewrite e; left; reflexivity. right.
+        intro F. inversion F; contradiction. right; discriminate.
+        left; apply ltfv_abs; assumption. right; intro F; inversion F; contradiction.
+      Defined.
+
+      Definition non_constant (C:Set) (x:T (^C)):= lt_free_variable (^C) None x.
+
+      Definition non_constant_test (C:Set) (x:T (^C)):
+        sumbool (lt_free_variable (^C) None x) (~lt_free_variable (^C) None x).
+      Proof.
+        apply lt_free_variable_test. intros. destruct w. right; discriminate.
+        left; reflexivity.
+      Defined.
+
+      Definition lt_i (C:Set):T C:= L C (V (^C) None).
+
+      Definition lt_constant_value (C:Set) (f: T (^C)): T C:=
+        lt_substitution (^C) f C (option_rect (fun _:^C => T C) (lt_var C) (lt_i C)).
+
+      Definition lt_constant_value_cov (C D:Set) (env: C -> D) (f: T (^C)):
+        lt_change_of_variables C (lt_constant_value C f) D env = 
+        lt_constant_value D (lt_change_of_variables (^C) f (^D) (option_map env)).
+      Proof.
+        unfold lt_constant_value. rewrite lt_sub_after_cov_equality.
+        rewrite lt_cov_after_sub_equality. apply lt_sub_pointwise_equality.
+        intros. destruct i; simpl; reflexivity.
+      Defined.
+        
+      Definition lt_constant_value_constant_embedding_equality (C:Set) (x: T C):
+        lt_constant_value C (lt_constant_embedding C x) = x.
+      Proof.
+        unfold lt_constant_value. unfold lt_constant_embedding.
+        rewrite lt_sub_after_cov_equality. simpl. apply lt_sub_identity_equality.
+      Defined.
+
+      Definition lt_sub_free_variable_pointwise_equality:
+        forall (C : Set) (f : T C) (D : Set) (env1 env2 : C -> T D),
+          (forall i : C, lt_free_variable C i f -> env1 i = env2 i) ->
+          lt_substitution C f D env1 = lt_substitution C f D env2.
+      Proof.
+        induction f. intros. simpl. apply H. apply ltfv_atom.
+        intros. simpl. rewrite IHf1 with (env2 := env2). rewrite IHf2 with (env2 := env2).
+        reflexivity. intros. apply H. apply ltfv_app_right; assumption.
+        intros. apply H. apply ltfv_app_left; assumption.
+        intros. simpl. apply f_equal. apply IHf. intros. destruct i. simpl. apply f_equal.
+        apply H. apply ltfv_abs; assumption. simpl; reflexivity.
+      Defined.
+        
+      Definition lt_constant_embedding_constant_value_equality (C:Set) (y: T (^C)):
+        ~non_constant C y ->
+        lt_constant_embedding C (lt_constant_value C y) = y.
+      Proof.
+        unfold lt_constant_value. unfold lt_constant_embedding. unfold non_constant.
+        rewrite lt_cov_after_sub_equality. intro.
+        rewrite lt_sub_free_variable_pointwise_equality with (env2 := lt_var (^C)).
+        apply lt_sub_identity_equality. intros. destruct i. simpl; reflexivity. contradiction.
+      Defined.
+
+      Lemma already_present_letters_cov (C:Set) (f: T C):
+        forall (D:Set) (env: C -> D) (w:D),
+          lt_free_variable D w (lt_change_of_variables C f D env) ->
+          exists v:C, (lt_free_variable C v f) /\ (env v = w).
+      Proof.
+        induction f. intros. inversion H. exists c. split. apply ltfv_atom. reflexivity.
+        simpl. intros. inversion H. apply IHf1 in H1. destruct H1 as (v1,pv1).
+        exists v1. split. apply ltfv_app_left; apply pv1. apply pv1.
+        apply IHf2 in H1. destruct H1 as (v2,pv2).
+        exists v2. split. apply ltfv_app_right; apply pv2. apply pv2.
+        simpl. intros. inversion H.  apply IHf in H1. destruct H1 as (o,po).
+        destruct po as (pol, por). destruct o. exists c. split. apply ltfv_abs; apply pol.
+        inversion por; reflexivity.  simpl in por; inversion por.
+      Defined.
+        
+      Definition lt_constant_embedding_is_constant (C:Set) (f: T C):
+        ~non_constant C (lt_constant_embedding C f).
+      Proof.
+        unfold non_constant. unfold lt_constant_embedding. intro F.
+        apply already_present_letters_cov in F. destruct F as (L,R). destruct R as (P,Q).
+        inversion Q.
+      Defined.      
+
+      Definition lt_free_variable_cov (C:Set) (v:C) (f:T C)
+                 (p:lt_free_variable C v f): forall (D:Set) (env: C -> D),
+          lt_free_variable D (env v) (lt_change_of_variables C f D env).
+      Proof.
+        induction p. simpl; intros; apply ltfv_atom.
+        simpl; intros; apply ltfv_app_left; apply IHp; assumption.
+        simpl; intros; apply ltfv_app_right; apply IHp; assumption.
+        simpl; intros; apply ltfv_abs. apply IHp with (env := option_map env).
+      Defined.
+
+      Definition non_constant_cov (C D:Set) (env: C -> D) (f: T (^C)):
+        non_constant C f <->
+        non_constant D (lt_change_of_variables (^C) f (^D) (option_map env)).
+      Proof.
+        unfold non_constant. split. intro p.
+        apply lt_free_variable_cov with (D:= ^D) (env := option_map env) in p.
+        simpl in p; assumption. intro q. destruct (non_constant_test C f) as [y|n].
+        assumption. apply lt_constant_embedding_constant_value_equality in n.
+        rewrite <- n in q. rewrite lt_constant_embedding_cov in q. 
+        apply lt_constant_embedding_is_constant in q. contradiction.
+      Defined.        
+
+      Lemma already_present_letters_sub (C:Set) (f: T C):
+        forall (D:Set) (env: C -> T D) (w:D),
+          lt_free_variable D w (lt_substitution C f D env) ->
+          exists i:C, (lt_free_variable C i f) /\(lt_free_variable D w (env i)).
+      Proof.
+        induction f. intros. exists c. split. apply ltfv_atom. simpl in H; assumption.
+        intros. simpl in H. inversion H.
+        apply IHf1 in H1. destruct H1 as (i1,p1). exists i1. split.
+        apply ltfv_app_left; apply p1. apply p1.
+        apply IHf2 in H1. destruct H1 as (i2,p2). exists i2. split.
+        apply ltfv_app_right; apply p2. apply p2.
+        intros. simpl in H. inversion H. apply IHf in H1.
+        destruct H1 as (i,pi). destruct i. exists c. split. apply ltfv_abs. apply pi.
+        simpl in pi. unfold lt_constant_embedding in pi.
+        destruct pi as (pir, pil). apply already_present_letters_cov in pil.
+        destruct pil as (iv, piv). destruct piv as (fiv, eiv). inversion eiv.
+        rewrite H2 in fiv; assumption. simpl in pi. destruct pi as (X,F). inversion F.
+      Defined.
+
+      Definition free_letters_in_specify_new_var (C:Set) (f:T (^C)) (t:T C) (v:C):
+        lt_free_variable C v (lt_specify_new_var C f t) ->
+        (lt_free_variable C v t) \/ (lt_free_variable (^C) (Some v) f).
+      Proof.
+        unfold lt_specify_new_var. unfold lt_set_new_variable. intro P.
+        apply already_present_letters_sub in P.
+        destruct P as (o, po). destruct po as (pol, por). destruct o. right. inversion por.
+        assumption. left; assumption.
+      Defined.
+      
+    End free_new_variables_and_constant_terms_characterizations.    
+    
+    Fixpoint max_pbed (C:Set) (x:T C) {struct x}: T C:=
+      match x as l return T C with
+      |V _ c => V _ c
+      |A _ y z => match y with
+                  | L _ f => lt_specify_new_var C (max_pbed (^C) f) (max_pbed C z)
+                  | _ => A C (max_pbed C y) (max_pbed C z)
+                  end
+      |L _ g => match g with
+                | A _ h (V _ None) => match (non_constant_test C h) with
+                                            | left _ => L C (max_pbed (^C) g)
+                                            | right _ =>
+                                              lt_constant_value C (max_pbed (^C) h)
+                                            end
+                | _ => L C (max_pbed (^C) g) 
+                end 
+      end.
+
+    Lemma lt_app_cov (C:Set) (f g:T C) (D:Set) (env: C -> D):
+        lt_change_of_variables C (A C f g) D env =
+        A D (lt_change_of_variables C f D env) (lt_change_of_variables C g D env).
+    Proof.
+      simpl; reflexivity.
+    Defined.
+    
+    Lemma lt_abs_cov (C:Set) (f:T (^C)) (D:Set) (env: C -> D):
+      lt_change_of_variables C (L C f) D env =
+      L D (lt_change_of_variables (^C) f (^D) (option_map env)).
+    Proof.
+      simpl; reflexivity.
+    Defined.
+
+    Fixpoint max_pbed_cov (C:Set) (f:T C) (D:Set) (env: C -> D) {struct f}:
+        lt_change_of_variables C (max_pbed C f) D env =
+        max_pbed D (lt_change_of_variables C f D env).
+    Proof.
+      destruct f. simpl; reflexivity.
+      assert (lt_change_of_variables C (max_pbed C f1) D env =
+              max_pbed D (lt_change_of_variables C f1 D env)) as R1. apply max_pbed_cov.
+      assert (lt_change_of_variables C (max_pbed C f2) D env =
+              max_pbed D (lt_change_of_variables C f2 D env)) as R2. apply max_pbed_cov.
+      destruct f1. simpl. rewrite R2.
+      reflexivity.
+      assert (forall (U:Set) (p q r: T U), max_pbed U (A U (A U p q) r) =
+                                           A U (max_pbed U (A U p q)) (max_pbed U r)
+             ) as E. intros; simpl; reflexivity. rewrite E. repeat rewrite lt_app_cov.
+      rewrite R1. rewrite E. rewrite lt_app_cov. rewrite R2. reflexivity.
+      simpl. rewrite lt_specify_new_var_cov. apply f_equal2. apply max_pbed_cov. apply R2.
+      assert (lt_change_of_variables (^C) (max_pbed (^C) f )(^D) (option_map env) =
+              max_pbed (^D) (lt_change_of_variables (^C) f (^D) (option_map env))
+             ) as R. apply max_pbed_cov.
+      destruct f. simpl; reflexivity. destruct f2. destruct o.
+      simpl; simpl in R; rewrite R. reflexivity. rewrite lt_abs_cov. rewrite lt_app_cov.
+      assert (lt_change_of_variables (^C) (V (^C) None) (^D) (option_map env)
+              = V (^D) None) as ENone. simpl; reflexivity. rewrite ENone.
+      simpl.
+      destruct (non_constant_test C f1).
+      destruct (non_constant_test D (lt_change_of_variables (^C) f1 (^D) (option_map env))).
+      simpl in R. rewrite <- R. rewrite lt_abs_cov. reflexivity. apply False_ind.
+      apply n. apply non_constant_cov. assumption.
+      destruct (non_constant_test D (lt_change_of_variables (^C) f1 (^D) (option_map env))).
+      apply False_ind. apply n. apply non_constant_cov in l. assumption.
+      rewrite lt_constant_value_cov. apply f_equal; apply max_pbed_cov.
+      simpl; simpl in R; rewrite R; reflexivity.
+      simpl; simpl in R; rewrite R; reflexivity.
+      simpl; simpl in R; rewrite R; reflexivity.
+    Defined.
+
+    Definition max_pbed_ce (C:Set) (x:T C):
+      lt_constant_embedding C (max_pbed C x) =
+      max_pbed (^C) (lt_constant_embedding C x).
+    Proof.
+      unfold lt_constant_embedding; apply max_pbed_cov.
+    Defined.
+    
+    Fixpoint pbed_towards_max (C:Set) (x:T C) {struct x}:
+      x §[C] max_pbed C x.
+    Proof.
+      destruct x. simpl; apply pbed_var_refl. simpl.
+      assert (x1 §[C] max_pbed C x1) as R1. apply pbed_towards_max.
+      assert (x2 §[C] max_pbed C x2) as R2. apply pbed_towards_max.
+      destruct x1. apply pbed_app. simpl; apply pbed_refl. assumption.
+      apply pbed_app; assumption. apply pbed_beta. apply pbed_towards_max. assumption.
+      assert (x §[^C] max_pbed (^C) x) as R. apply pbed_towards_max.
+      destruct x. simpl; apply pbed_refl. destruct x2. destruct o.
+      simpl. apply pbed_abs. simpl in R. assumption. simpl.
+      destruct (non_constant_test C x1). simpl in R. apply pbed_abs; assumption.
+      assert (L C (A (^C) x1 (V (^C) None)) =
+              L C (A (^C) (lt_constant_embedding C (lt_constant_value C x1)) (V (^C) None))
+             ) as Ecvce.
+      rewrite <- lt_constant_embedding_constant_value_equality with (y:=x1).
+      rewrite lt_constant_value_constant_embedding_equality. reflexivity. assumption.
+      rewrite Ecvce. apply pbed_eta. unfold lt_constant_value. apply pbed_sub.
+      apply pbed_towards_max. intros. apply pbed_refl. 
+      simpl. apply pbed_abs. simpl in R. assumption.
+      simpl. apply pbed_abs. simpl in R. assumption.
+      simpl. apply pbed_abs. simpl in R. assumption.
+    Defined.                   
+    
+  End the_maximum_direct_reduction_operator.
+
+  Lemma lt_app_sub (C:Set) (f g:T C) (D:Set) (env: C -> T D):
+    lt_substitution C (A C f g) D env =
+    A D (lt_substitution C f D env) (lt_substitution C g D env).
+  Proof.
+    simpl; reflexivity.
+  Defined.
+
+  Lemma lt_app_specify_new_var (C:Set) (f g:T (^ C)) (t:T C):
+    lt_specify_new_var C (A (^C) f g) t =
+    A C (lt_specify_new_var C f t) (lt_specify_new_var C g t).
+  Proof.
+    apply lt_app_sub. 
+  Defined.  
+
+  Fixpoint no_letter_added_by_reduction
+           (C:Set) (x y:T C) (r: x§[C] y) {struct r}:
+    forall (v:C), lt_free_variable C v y -> lt_free_variable C v x.
+  Proof.
+    destruct r. intros. assumption. intros v Fv. inversion Fv.
+    apply ltfv_app_left. apply no_letter_added_by_reduction with (v:=v) in r1; assumption.
+    apply ltfv_app_right. apply no_letter_added_by_reduction with (v:=v) in r2; assumption.
+    intros v Fv. inversion Fv.
+    apply ltfv_abs; apply no_letter_added_by_reduction with (v:= Some v) in r; assumption.
+    intros v Fv. apply free_letters_in_specify_new_var in Fv.
+    destruct Fv as [Fvl|Fvr]. apply no_letter_added_by_reduction with (v:=v) in r2.
+    apply ltfv_app_right. assumption. assumption.
+    apply no_letter_added_by_reduction with (v:=Some v) in r1. apply ltfv_app_left.
+    apply ltfv_abs; assumption. assumption.
+    intros v Fv. apply no_letter_added_by_reduction with (v:=v) in r.
+    apply ltfv_abs. apply ltfv_app_left. unfold lt_constant_embedding.
+    apply lt_free_variable_cov. assumption. assumption.
+  Defined.  
+
+  Corollary reduction_of_constants (C:Set) (x y: T (^C)):
+    (~ non_constant C x) ->
+    x §[^C] y ->
+    ~ non_constant C y.
+  Proof.
+    unfold non_constant. intros. intro. apply H.
+    apply no_letter_added_by_reduction with (v:= None) in H0; assumption.
+  Defined.
+  
+  Fixpoint Takahashi_confluence_trick (C:Set) (f: T C) {struct f}:
+    forall (g: T C), f §[C] g ->
+                     g §[C] max_pbed C f.
+  Proof.
+    destruct f. intros g R. inversion R. simpl; apply pbed_var_refl. 
+    assert (forall k:T C, f1 §[C] k -> k §[C] max_pbed C f1) as Q1.
+    apply Takahashi_confluence_trick; assumption.
+    assert (forall k:T C, f2 §[C] k -> k §[C] max_pbed C f2) as Q2.
+    apply Takahashi_confluence_trick; assumption. intros g R. inversion R.
+    destruct f1. simpl. apply pbed_app. apply Q1; assumption. simpl. apply Q2; assumption.
+    simpl. destruct f1_1. inversion H1.
+    apply pbed_app. apply Q1. rewrite H7; assumption. apply Q2; assumption. apply pbed_app.
+    apply Q1; assumption. apply Q2; assumption.
+    apply pbed_app. apply Q1; assumption. apply Q2; assumption.
+    assert (forall k:T (^C), f1 §[^C] k -> k §[^C] max_pbed (^C) f1) as Q1'.
+    apply Takahashi_confluence_trick; assumption. simpl. inversion H1.
+    apply pbed_beta. apply Q1'; assumption. apply Q2; assumption.
+    assert (A C a' b' = lt_specify_new_var C (A (^C) (lt_constant_embedding C a')
+                                                (V (^C) None)) b') as Ea'.
+    rewrite lt_app_specify_new_var. rewrite lt_specify_new_var_constant.
+    unfold lt_specify_new_var; simpl; reflexivity. rewrite Ea'. apply pbed_specify_new_var.
+    rewrite <- H4 in Q1'. apply Q1'. apply pbed_app. apply pbed_cov; assumption.
+    apply pbed_var_refl. apply Q2; assumption. simpl.
+    apply pbed_specify_new_var.
+    destruct f1. inversion H. inversion H. 
+    assert (forall k:T (^C), f1 §[^C] k -> k §[^C] max_pbed (^C) f1) as Q.
+    apply Takahashi_confluence_trick. inversion H. rewrite H5 in H1. apply Q in H1.
+    assumption. apply Q2; assumption.
+    intros. 
+    assert (forall k:T (^C), f §[^C] k -> k §[^C] max_pbed (^C) f) as Q'.
+    apply Takahashi_confluence_trick.
+    destruct f. simpl. inversion H. inversion H1. apply pbed_refl. 
+    assert (forall k:T (^C), f1 §[^C] k -> k §[^C] max_pbed (^C) f1) as Q1'.
+    apply Takahashi_confluence_trick.
+    assert (forall k:T (^C), f2 §[^C] k -> k §[^C] max_pbed (^C) f2) as Q2'.
+    apply Takahashi_confluence_trick.
+    destruct f2. destruct o. inversion H. simpl. apply pbed_abs; apply Q'; assumption.
+    simpl. destruct (non_constant_test C f1).
+    inversion H. simpl. apply pbed_abs; apply Q'; assumption.
+    apply False_rect. apply (lt_constant_embedding_is_constant C f). rewrite <- H0 in l.
+    assumption. destruct f1.    
+    inversion H. inversion H1. inversion H5. inversion H7. unfold lt_constant_value.
+    destruct o. simpl. apply pbed_eta with (f:= V C c). apply pbed_refl. simpl.
+    apply False_rect. apply n. apply ltfv_atom. rewrite H0.
+    apply f_equal with (f:= lt_constant_value C) in H0.
+    rewrite lt_constant_value_constant_embedding_equality in H0. rewrite H0 in H1.
+    destruct o. unfold lt_constant_value. unfold lt_constant_value in H1. simpl in H1.
+    simpl. inversion H1; apply pbed_var_refl. apply False_rect. apply n; apply ltfv_atom.
+    assert (forall k:T (^C), f1_1 §[^C] k -> k §[^C] max_pbed (^C) f1_1) as Q1_1'.
+    apply Takahashi_confluence_trick.
+    assert (forall k:T (^C), f1_2 §[^C] k -> k §[^C] max_pbed (^C) f1_2) as Q1_2'.
+    apply Takahashi_confluence_trick. inversion H. inversion H1. inversion H7.
+    assert (lt_constant_embedding C (lt_constant_value C a') = a') as Ea'.
+    apply lt_constant_embedding_constant_value_equality.
+    apply reduction_of_constants with (x:= A (^C) f1_1 f1_2); assumption. rewrite <- Ea'.
+    apply pbed_eta. unfold lt_constant_value; apply pbed_sub. apply Q1'. assumption.
+    intros; apply pbed_refl.
+    apply pbed_ce in H1. rewrite H0 in H1. apply Q1' in H1. 
+    rewrite <- lt_constant_value_constant_embedding_equality with (x:= g).
+    unfold lt_constant_value; apply pbed_sub. rewrite H0; assumption. intros; apply pbed_refl.
+    assert (forall k:T (^^C), f1 §[^^C] k -> k §[^^C] max_pbed (^^C) f1) as Q1''.
+    apply Takahashi_confluence_trick. inversion H. inversion H1. inversion H7. 
+    assert (lt_constant_embedding C (lt_constant_value C a') = a') as Ea'.
+    apply lt_constant_embedding_constant_value_equality.
+    apply reduction_of_constants with (x:= L (^C) f1); assumption. rewrite <- Ea'.
+    apply pbed_eta. unfold lt_constant_value; apply pbed_sub. apply Q1'. assumption.
+    intros; apply pbed_refl. inversion H7.
+    rewrite <- lt_constant_value_constant_embedding_equality with
+        (x:= L C (lt_specify_new_var (^ C) f'0 (V (^ C) None))). unfold lt_constant_value.
+    apply pbed_sub. apply Q1'. unfold lt_constant_embedding. simpl.
+    apply pbed_abs. unfold lt_specify_new_var. rewrite lt_cov_after_sub_equality.
+    assert (lt_substitution (^^C) f1 (^^C) (lt_var (^^C)) =
+            lt_substitution
+              (^^ C) f1 (^^ C)
+              (fun i : ^^ C =>
+                 lt_change_of_variables (^ C) (lt_set_new_variable (^ C) (V (^ C) None) i)
+                                        (^ (^ C)) (option_map Some))
+           ) as Ef1.
+    apply lt_sub_free_variable_pointwise_equality. intros. destruct i.
+    destruct o. simpl. reflexivity. apply False_rect. apply n. apply ltfv_abs; assumption.
+    simpl; reflexivity. rewrite lt_sub_identity_equality in Ef1. rewrite Ef1. apply pbed_sub.
+    assumption. intros; apply pbed_refl. intros; apply pbed_refl. 
+    apply pbed_ce in H1. rewrite H0 in H1. apply Q1' in H1. 
+    rewrite <- lt_constant_value_constant_embedding_equality with (x:= g).
+    unfold lt_constant_value; apply pbed_sub. rewrite H0; assumption. intros; apply pbed_refl.
+    inversion H. simpl. apply pbed_abs. apply Q'; assumption.
+    inversion H. simpl. apply pbed_abs. apply Q'; assumption. 
+    inversion H. simpl. apply pbed_abs. apply Q'; assumption.
+  Defined.
+
+  Definition pbed_confluence (C:Set) (x a b:T C):
+    (x §[C] a) -> (x§[C] b) -> {y:T C & prod (a §[C] y) (b §[C] y)}.
+  Proof.
+    intros ra rb. exists (max_pbed C x). split; apply Takahashi_confluence_trick; assumption.
+  Defined.  
+
+  Fixpoint pbe_pbed_semi_confluence (C:Set) (x a:T C) (r: x §*[C] a) (b:T C) (s: x §[C] b)
+           {struct r}:
+     {y:T C & prod (a §[C] y) (b §*[C] y)}.
+  Proof.
+    destruct r. exists b. split. assumption. apply pbe_refl.
+    apply pbe_pbed_semi_confluence with (b:=b) in r.
+    destruct r as (w,pw). apply pbed_confluence with (b:= w) in p. destruct p as (v,pv).
+    exists v. split. apply pv. apply pbe_step with (y:= w). apply pw. apply pv. apply pw.
+    assumption.
+  Defined.
+
+  Fixpoint pbe_confluence (C:Set) (x a:T C) (r: x §*[C] a) (b:T C) (s: x §*[C] b)
+           {struct r}:
+     {y:T C & prod (a §*[C] y) (b §*[C] y)}.
+  Proof.
+    destruct r. exists b. split. assumption. apply pbe_refl.
+    apply pbe_confluence with (b:=b) in r.
+    destruct r as (w,pw). apply pbe_pbed_semi_confluence with (a:= w) in p.
+    destruct p as (v,pv).
+    exists v. split. apply pv. apply pbe_step with (y:= w). apply pw. apply pv. apply pw.
+    assumption.
+  Defined.
+    
+End Takahashi_reductions_and_their_confluence.
+
+Section equivalence_between_Takahashi_and_usual_reduction_and_confluence_of_the_latter.
+
+  Notation T:= Lambda_Term.
+  Notation V:= lt_var.
+  Notation A:= lt_app.
+  Notation L:= lt_abs.
+  Notation "^ C":= (option C) (right associativity, at level 41).
+
+  Notation "a §[ C ] b":= (parallel_beta_eta_direct_reduction C a b) (at level 49).
+  Notation "a §*[ C ] b":= (parallel_beta_eta_reduction C a b) (at level 49).
+
+  Notation "a >[ C ] b":= (lt_beta_eta_reduction C a b) (at level 49).
+  
+  Section good_behavior_of_beta_eta_reduction_under_change_of_variables_and_substitution.
+
+    Definition ltber_cov (C:Set) (x y:T C) (r: x >[C] y):
+      forall (D:Set) (env: C -> D),
+        (lt_change_of_variables C x D env) >[D] (lt_change_of_variables C y D env).
+    Proof.
+      induction r. intros; simpl; rewrite lt_specify_new_var_cov; apply ltber_redex.
+      intros; simpl; rewrite lt_constant_embedding_cov; apply ltber_eta.
+      intros; simpl; apply ltber_app. apply IHr1. apply IHr2.
+      intros; simpl; apply ltber_abs; apply IHr. intros; apply ltber_reflexivity.
+      intros; simpl; apply ltber_transitivity with (y:= lt_change_of_variables C y D env).
+      apply IHr1. apply IHr2.
+    Defined.
+
+    Notation ce:= (lt_constant_embedding).
+    
+    Definition ltber_ce (C:Set) (x y:T C) (r: x >[C] y): (ce C x) >[^C] (ce C y):=
+      ltber_cov C x y r (^ C) Some.
+    
+    Definition ltber_sub (C:Set) (x y:T C) (r: x >[C] y):
+      forall (D:Set) (env: C -> T D),
+        (lt_substitution C x D env) >[D] (lt_substitution C y D env).
+    Proof.
+      induction r. intros; simpl. rewrite lt_specify_new_var_sub; apply ltber_redex.
+      intros. simpl. rewrite lt_constant_embedding_sub. apply ltber_eta.
+      intros; simpl; apply ltber_app. apply IHr1; assumption. apply IHr2; assumption.
+      intros; simpl; apply ltber_abs; apply IHr; assumption.
+      intros; apply ltber_reflexivity.
+      intros; simpl; apply ltber_transitivity with (y:= lt_substitution C y D env).
+      apply IHr1. apply IHr2.
+    Defined.
+
+    Definition ltber_env (C:Set) (x:T C):
+      forall (D:Set) (env1 env2: C -> T D) (redenv: forall i:C, env1 i >[D] env2 i),
+        (lt_substitution C x D env1) >[D] (lt_substitution C x D env2).
+    Proof.
+      induction x. intros; simpl; apply redenv. intros; simpl; apply ltber_app.
+      apply IHx1; assumption. apply IHx2; assumption.
+      intros; simpl; apply ltber_abs; apply IHx. intros. destruct i.
+      simpl; apply ltber_ce; apply redenv. simpl; apply ltber_reflexivity.
+    Defined.
+      
+    Definition ltber_parallel_sub (C:Set) (x y:T C) (r: x >[C] y):
+      forall (D:Set) (env1 env2: C -> T D) (redenv: forall i:C, env1 i >[D] env2 i),
+        (lt_substitution C x D env1) >[D] (lt_substitution C y D env2).
+    Proof.
+      intros. apply ltber_transitivity with (y:= lt_substitution C y D env1).
+      apply ltber_sub; assumption. apply ltber_env; apply redenv.
+    Defined.
+    
+    Definition ltber_parallel_specify_new_var (C:Set) (f f': T (^C)) (x x':T C):
+      f >[^C] f' -> x >[C] x' -> lt_specify_new_var C f x >[C] lt_specify_new_var C f' x'.
+    Proof.
+      intros; unfold lt_specify_new_var; apply ltber_parallel_sub. assumption.
+      intros; destruct i; simpl. apply ltber_reflexivity. assumption.
+    Defined.      
+
+    Definition ltber_parallel_beta (C:Set) (f f':T (^C)) (x x':T C):
+      f >[^C] f' -> x >[C] x' -> A C (L C f) x >[C] lt_specify_new_var C f' x'.
+    Proof.
+      intros; apply ltber_transitivity with (y:= lt_specify_new_var C f x).
+      apply ltber_redex. apply ltber_parallel_specify_new_var; assumption.
+    Defined.
+
+    Definition ltber_parallel_eta (C:Set) (f f':T C):
+      f >[C] f' -> L C (A (^C) (lt_constant_embedding C f) (V (^C) None)) >[C] f'.
+    Proof.
+      intros; apply ltber_transitivity with (y:= f). apply ltber_eta; assumption. assumption.
+    Defined.
+      
+  End good_behavior_of_beta_eta_reduction_under_change_of_variables_and_substitution.
+ 
+  Section further_properties_of_parallel_beta_eta_reduction.
+    
+    Definition pbed_to_pbe (C:Set) (x y:T C):
+      x §[C] y -> x §*[C] y.
+    Proof.
+      intros. apply pbe_step with (y:=x). apply pbe_refl. assumption.
+    Defined.
+
+    Definition pbe_transitivity (C:Set) (y z:T C) (r: y §*[C] z):
+      forall (x: T C), x §*[C] y -> x §*[C] z.
+      induction r. intros; assumption. intros. apply pbe_step with (y:=y).
+      apply IHr; assumption. assumption.
+    Defined.
+
+    Definition pbe_left (C:Set) (x a b:T C) (r: a §*[C] b):
+      (A C a x) §*[C] (A C b x).
+    Proof.
+      induction r. apply pbe_refl. apply pbe_step with (y:= A C y x). assumption.
+      apply pbed_app. assumption. apply pbed_refl.
+    Defined.
+
+    Definition pbe_right (C:Set) (x a b:T C) (r: a §*[C] b):
+      (A C x a) §*[C] (A C x b).
+    Proof.
+      induction r. apply pbe_refl. apply pbe_step with (y:= A C x y). assumption.
+      apply pbed_app. apply pbed_refl. assumption.
+    Defined.
+      
+    Definition pbe_app (C:Set) (x x' y y':T C):
+      x §*[C] x' -> y §*[C] y' -> (A C x y) §*[C] (A C x' y').
+    Proof.
+      intros. apply pbe_transitivity with (y:= A C x' y). apply pbe_right; assumption.
+      apply pbe_left; assumption.
+    Defined.
+
+    Definition pbe_abs (C:Set) (x y:T (^C)) (r: x §*[^C] y):
+      L C x §*[C] L C y.
+    Proof.
+      induction r. apply pbe_refl. apply pbe_step with (y:= L C y). assumption.
+      apply pbed_abs. assumption.
+    Defined.      
+      
+  End further_properties_of_parallel_beta_eta_reduction.
+    
+  Section equivalence_between_the_two_reductions.
+
+    Ltac tr := apply pbed_to_pbe.
+
+    Definition pbed_to_ltber (C:Set) (x y:T C) (r: parallel_beta_eta_direct_reduction C x y):
+      lt_beta_eta_reduction C x y.
+    Proof.
+      induction r. apply ltber_reflexivity. apply ltber_app; assumption.
+      apply ltber_abs; assumption. apply ltber_parallel_beta; assumption.
+      apply ltber_parallel_eta; assumption.
+    Defined.
+
+    Definition pbe_to_ltber (C:Set) (x y:T C) (r: parallel_beta_eta_reduction C x y):
+      lt_beta_eta_reduction C x y.
+    Proof.
+      induction r. apply ltber_reflexivity. apply ltber_transitivity with (y:=y).
+      assumption. apply pbed_to_ltber; assumption.
+    Defined.
+
+    Definition ltber_to_pbe (C:Set) (x y:T C) (r: lt_beta_eta_reduction C x y):
+      parallel_beta_eta_reduction C x y.      
+    Proof.
+      induction r. tr; apply pbed_beta; apply pbed_refl. tr; apply pbed_eta; apply pbed_refl. 
+      apply pbe_app; assumption. apply pbe_abs; assumption. apply pbe_refl.
+      apply pbe_transitivity with (y:= y); assumption.
+    Defined.
+            
+  End equivalence_between_the_two_reductions.
+
+  Section the_Church_Rosser_for_beta_eta_reduction_in_lambda_calculus.
+
+    Definition ltber_confluence (C:Set) (x a:T C) (r: x >[C] a) (b:T C) (s: x >[C] b):
+      {y:T C & prod (a >[C] y) (b >[C] y)}.
+    Proof.
+      apply ltber_to_pbe in r. apply ltber_to_pbe in s.
+      destruct (pbe_confluence C x a r b s) as (m,p). exists m.
+      split; apply pbe_to_ltber; apply p.
+    Defined.    
+
+  End the_Church_Rosser_for_beta_eta_reduction_in_lambda_calculus.  
+  
+End equivalence_between_Takahashi_and_usual_reduction_and_confluence_of_the_latter.
