naslc_library.v
@@ -1,0 +1,1 @@
+Require Export NasLC.nested_abstract_syntax_lambda_calculus NasLC.confluence_of_lambda_calculus_according_to_takahashi.
